\batchmode
\documentclass{article}
\usepackage{epsfig}
% Packages requested by user
\usepackage{amsmath}
\usepackage{amsfonts}

\pagestyle{empty}
\begin{document}
$\ldots$
\pagebreak

$ \ldots $
\pagebreak

$ 1- $
\pagebreak

$ i $
\pagebreak

$ j $
\pagebreak

$ k $
\pagebreak

$ [i:j] $
\pagebreak

$ [k:l] $
\pagebreak

$ i-j $
\pagebreak

$ k-l $
\pagebreak

$ (i,j), \ldots, (i+(k-1), j-(k-1)) $
\pagebreak

$ p \in [i:j] $
\pagebreak

$ q \in [k:l] $
\pagebreak

$ (i,j) $
\pagebreak

$ (p,q) $
\pagebreak

$ i < p < j < q $
\pagebreak

$ p < i < q < j $
\pagebreak

$ E_{ij} $
\pagebreak

\[ E_{ij} = \min \left[ \max_{(i,k) \in \{GC, CG, AU, UA, GU, UG\}} E_{ik}, \max_{(k,j) \in \{GC, CG, AU, UA, GU, UG\}} E_{kj} \right]. \]
\pagebreak

$ e $
\pagebreak

$ kcal / mol $
\pagebreak

$ m $
\pagebreak

$ -5 kcal/mol $
\pagebreak

$p(s)$
\pagebreak

$s$
\pagebreak

$E(s)$
\pagebreak

\[ p(s) \propto e^{-\beta E(s)} \text{ with } \beta = \frac{1}{kT} \]
\pagebreak

$k \approx 1.987 \cdot 10^{-3} \frac{kcal}{mol~K}$
\pagebreak

$T$
\pagebreak

\[ Z = \sum_{s \in \Omega} e^{-\beta E(s)} \]
\pagebreak

$\Omega$
\pagebreak

\[ p(s) = \frac{e^{-\beta E(s)}}{Z} \]
\pagebreak

$Z$
\pagebreak

$q1k(k) = Q(1, k)$
\pagebreak

$qln(l) = Q(l, n)$
\pagebreak

$ <d(S)> = \sum_{(i,j) \in S} (1-p_{ij}) + \sum_{(i,j) \notin S} p_{ij} $
\pagebreak

$p_ij>0.5$
\pagebreak

$k$
\pagebreak

$<d> = \sum_{a,b} p_a p_b d(S_a,S_b)$
\pagebreak

$p_ij$
\pagebreak

$<d> = \sum_{ij} p_{ij}(1-p_{ij})$
\pagebreak

$(i,j)$
\pagebreak

$(i+1, j-1)$
\pagebreak

$ p > \textrm{cutoff} $
\pagebreak

$ p $
\pagebreak

\[ p(s) = \frac{exp(-\beta E(s)}{Z} \]
\pagebreak

\[ Z = \sum_s exp(-\beta E(s)),\quad\mathrm{with}\quad\beta = \frac{1}{RT} \]
\pagebreak

$R$
\pagebreak

$[0:1]$
\pagebreak

$ \ge 1 $
\pagebreak

$E$
\pagebreak

$10 cal/mol$
\pagebreak

$q = exp(-\beta E)$
\pagebreak

$\beta = \frac{1}{RT}$
\pagebreak

$E_{max}$
\pagebreak

$E_{saddle} < E_{max}$
\pagebreak

$\Sigma$
\pagebreak

$ \Sigma = \{A,U,C,G\} $
\pagebreak

$\mathrm{strlen}(\mathrm{sequence})+1$
\pagebreak

$-kT \cdot \log(p)$
\pagebreak

$p$
\pagebreak

\[ A(S) = \sum_{(i,j) \in S} 2 \gamma p_{ij} + \sum_{i \notin S} p^u_i \]
\pagebreak

$\gamma$
\pagebreak

$ exp(-E / (b \cdot kT))$
\pagebreak

$exp{((-F/kT)/length)}$
\pagebreak

$F$
\pagebreak

$Q$
\pagebreak

$G = -RT \cdot \log(Q) $
\pagebreak

$\Delta G = - RT \ln Z$
\pagebreak

$ N \times M $
\pagebreak

$N$
\pagebreak

$M$
\pagebreak

$X[100][5]$
\pagebreak

$ F(\vec\epsilon) = \sum_{i = 1}^n{ \frac{\epsilon_i^2}{\tau^2} } + \sum_{i = 1}^n{ \frac{(p_i(\vec\epsilon) - q_i)^2}{\sigma^2} } \to min $
\pagebreak

$ F(\vec\epsilon) = \sum_{i = 1}^n{ \frac{|\epsilon_i|}{\tau^2} } + \sum_{i = 1}^n{ \frac{|p_i(\vec\epsilon) - q_i|}{\sigma^2} } \to min $
\pagebreak

\[ F(\vec\epsilon) = \sum_{\mu}{ \frac{\epsilon_{\mu}^2}{\tau^2} } + \sum_{i = 1}^n{ \frac{(p_i(\vec\epsilon) - q_i)^2}{\sigma^2} } \to \min. \]
\pagebreak

$ 1~J = 1~kg \cdot m^2 s^{-2} $
\pagebreak

$ 1~kJ = 1,000~J $
\pagebreak

$ 1~cal_{IT} = 4.1868~J $
\pagebreak

$ 1~dacal_{IT} = 10~cal_{IT} = 41.868~J $
\pagebreak

$ 1~kcal_{IT} = 4.1868~kJ $
\pagebreak

$ 1~cal_{th} = 4.184~J $
\pagebreak

$ 1~dacal_{th} = 10~cal_{th} = 41.84~J $
\pagebreak

$ 1~kcal_{th} = 4.184~kJ $
\pagebreak

$ 1~g~\mathrm{TNT} = 1,000~cal_{th} = 4,184~J $
\pagebreak

$ 1~kg~\mathrm{TNT} = 1,000~kcal_{th} = 4,184~kJ $
\pagebreak

$ 1~t~\mathrm{TNT} = 1,000,000~kcal_{th} = 4,184~MJ $
\pagebreak

$ 1~eV = 1.602176565 \times 10^{-19}~J $
\pagebreak

$ 1~W \cdot h = 1~W \cdot 3,600 s = 3,600~J = 3.6~kJ $
\pagebreak

$ 1~kW \cdot h = 1~kW \cdot 3,600~s = 3,600~kJ = 3.6~MJ $
\pagebreak

$ [^{\circ}C] = [K] - 273.15 $
\pagebreak

$ [^{\circ}F] = [K] \times \frac{9}{5} - 459.67 $
\pagebreak

$ [^{\circ}R] = [K] \times \frac{9}{5} $
\pagebreak

$ [^{\circ}N] = ([K] - 273.15) \times \frac{33}{100} $
\pagebreak

$ [^{\circ}De] = (373.15 - [K]) \time \frac{3}{2} $
\pagebreak

$ [^{\circ}R{\acute e}] = ([K] - 273.15) \times \frac{4}{5} $
\pagebreak

$ [^{\circ}\mathrm{R{\o}}] = ([K] - 273.15) \times \frac{21}{40} + 7.5 $
\pagebreak

$f(i,j)$
\pagebreak

$[i,j]$
\pagebreak

$i$
\pagebreak

$j$
\pagebreak

$ [i,j] $
\pagebreak

$ exp(-E / kT) $
\pagebreak

$ E $
\pagebreak

$\hat{q}[i,j] = q[i,j] / s^{(j-i+1)}$
\pagebreak

$ s = exp((sfact * MFE) / kT / length )$
\pagebreak

$ exp(-\Delta G / kT) $
\pagebreak

$ e^{-E/(\alpha \cdot K \cdot T)} $
\pagebreak

$\Delta G$
\pagebreak

$10^{-2} * \mathrm{kcal}/\mathrm{mol}$
\pagebreak

$e^{-\Delta G/kT} $
\pagebreak

$(i - 1)$
\pagebreak

$(j+1)$
\pagebreak

$-1$
\pagebreak

$size + 2$
\pagebreak

$(k,l)$
\pagebreak

$(n+m)$
\pagebreak

$[i:j]$
\pagebreak

$[i:k]$
\pagebreak

$[l:j]$
\pagebreak

$[k:l]$
\pagebreak

$(l,j)$
\pagebreak

$(i,k)$
\pagebreak

$(l,j-1)$
\pagebreak

$ d < 0 $
\pagebreak

$ d > 0 $
\pagebreak

$ d == 0 $
\pagebreak

$k_d = 0.32 \mu mol / l $
\pagebreak

\[ \Delta G_{\text{SHAPE}}(i) = m \ln(\text{SHAPE reactivity}(i)+1)+ b \]
\pagebreak

$ b $
\pagebreak

$ q_i $
\pagebreak

\[ \Delta G_{\text{SHAPE}}(x,i) = \beta\ |x_i - q_i| \]
\pagebreak

$ x_i=0 $
\pagebreak

$ x_i=1 $
\pagebreak

$ \beta $
\pagebreak

$ |x_i - q_i| $
\pagebreak

$ \hat{E} $
\pagebreak

$ dacal/mol $
\pagebreak

$ 1 dacal/mol = 10 cal/mol $
\pagebreak

$ exp(- \hat{E} / kT) $
\pagebreak

$ cal/mol $
\pagebreak

$P^t$
\pagebreak

$rs$
\pagebreak

$[0,1]$
\pagebreak

$ P^{t}_x[i] = X[i] * rs$
\pagebreak

$P^{t}_y[i] = Y[i] * rs$
\pagebreak

$ H = - \sum_c p_c \cdot \log_2 p_c $
\pagebreak

$ p(i,j) = S_i + S_j - p_ij*ln(p_ij) $
\pagebreak

$x == y $
\pagebreak

$2^b -1$
\pagebreak

$ 1 \leq i < j \leq n $
\pagebreak

$i $
\pagebreak

$ 1 \leq i \leq n $
\pagebreak

\end{document}
